Prove more of ctr.Client.Get() using prophecy.
Interestingly, it seems like we don't need to prophecize about whether
the epoch number is stale or not. If it is stale, the code will
physically return an error, and we Exit().

src/program_proof/fencing/ctr_proof.v
@@ -28,7 +28,8 @@ Implicit Type γ : ctr_names.
 Class ctrG Σ :=
   { mnat_inG:> mono_natG Σ;
     val_inG:> mapG Σ u64 u64;
-    unused_tok_inG:> mapG Σ u64 bool
+    unused_tok_inG:> mapG Σ u64 bool;
+    tok_inG :> inG Σ (dfracR)
   }.
 
 Context `{!ctrG Σ}.
@@ -156,29 +157,58 @@ else (* XXX: it might seem like the server shouldn't need any resources in this 
    (own_latest_epoch γ latestEpoch (1/2)%Qp ={↑ctrN, ⊤}=∗ Φ))
 .
 
-(* In this spec:
-   If the server can prove to the client that latestEpoch < e, then the client
-   needs to give back to the server the own_latest_epoch and own_unused_epoch
-   under a view-shift and the client will get back own_val of the new epoch, and
-   the previous latest epoch.
-
-   I think this might not be strictly TaDa.
- *)
-Definition EnterNewEpoch_spec' γ (e:u64) (Φ:iProp Σ) : iProp Σ :=
-∀ latestEpoch, own_latest_epoch γ latestEpoch (1/2)%Qp -∗
-if decide (int.Z latestEpoch < int.Z e)%Z then
-  |={⊤, ∅}=> own_latest_epoch γ latestEpoch (1)%Qp ∗ own_unused_epoch γ e ∗
-            (∀ v, own_val γ e v (1/2)%Qp -∗
-                  own_val γ latestEpoch v (1/2)%Qp -∗
-                  own_latest_epoch γ e (1/2)%Qp ={∅,⊤}=∗ Φ)
-else
-  Φ
+Lemma EnterNewEpoch_spec_wand γ e Φ1 Φ2 :
+  (Φ1 -∗ Φ2) -∗
+  EnterNewEpoch_spec γ e Φ1 -∗
+  EnterNewEpoch_spec γ e Φ2
 .
+Proof.
+  iIntros "Hwand Hupd".
+  rewrite /EnterNewEpoch_spec.
+  iMod "Hupd".
+  iDestruct "Hupd" as (?) "Hupd".
+  iExists latestEpoch.
+  destruct (decide (_)).
+  {
+    iModIntro.
+    iDestruct "Hupd" as "($ & $ & Hupd)".
+    iIntros (v) "H1 H2 H3".
+    iApply "Hwand".
+    iMod ("Hupd" $! v with "H1 H2 H3") as "$".
+    done.
+  }
+  {
+    iModIntro.
+    iDestruct "Hupd" as "[$ Hupd]".
+    iIntros "H1".
+    iApply "Hwand".
+    by iApply "Hupd".
+  }
+Qed.
 
 Definition Get_core_spec γ (e:u64) (Φ:u64 → iProp Σ) : iProp Σ :=
-  |={∅}=> ∃ v, own_val γ e v (1/2)%Qp ∗
+  |={∅}=> ∃ v, own_val γ e v (1/2)%Qp ∗ (* XXX: have a ∅ here because this runs inside of a larger atomic step *)
     (own_val γ e v (1/2)%Qp ={∅}=∗ (Φ v))
 .
+
+Lemma Get_core_spec_wand γ e Φ1 Φ2 :
+  (∀ x, Φ1 x -∗ Φ2 x) -∗
+  Get_core_spec γ e Φ1 -∗
+  Get_core_spec γ e Φ2
+.
+Proof.
+  iIntros "Hwand Hupd".
+  rewrite /Get_core_spec.
+  iMod "Hupd".
+  iModIntro.
+  iDestruct "Hupd" as (v) "Hupd".
+  iExists v.
+  iDestruct "Hupd" as "[$ Hupd]".
+  iIntros "H1".
+  iApply "Hwand".
+  iApply "Hupd".
+  iFrame.
+Qed.
 
 Definition Get_server_spec γ (e:u64) (Φ:u64 → u64 → iProp Σ) : iProp Σ :=
 |={⊤,∅}=> ∃ latestEpoch, own_latest_epoch γ latestEpoch (1/2)%Qp ∗
@@ -275,7 +305,8 @@ Definition getN := nroot .@ "ctr.get".
 
 Implicit Types γreq : gname.
 
-Definition operation_receipt γreq : iProp Σ := True.
+Definition operation_unfinished γreq : iProp Σ := own γreq (DfracOwn 1).
+Definition operation_receipt γreq : iProp Σ := own γreq (DfracDiscarded).
 
 Definition Get_req_inv prophV prophErr e γ γreq Φ : iProp Σ :=
   inv getN (
@@ -284,8 +315,8 @@ Definition Get_req_inv prophV prophErr e γ γreq Φ : iProp Σ :=
            prophV, but it's convenient to just reuse the more powerful spec definition.
          *)
     (EnterNewEpoch_spec γ e
-        (Get_server_spec γ e (λ v err, Φ v err)%I)) ∨
-    (Get_server_spec γ e (λ v err, (∀ l, ⌜has_GetReply_encoding l err v⌝ -∗ Φ err v)%I)) ∨
+        (Get_server_spec γ e (λ v err, Φ v err)) ∗ operation_unfinished γreq) ∨
+    (Get_server_spec γ e (λ v err, (∀ l, ⌜has_GetReply_encoding l err v⌝ -∗ Φ err v)%I) ∗ operation_unfinished γreq) ∨
     (Φ prophErr prophV) ∗ operation_receipt γreq)
 .
 
@@ -359,67 +390,54 @@ Proof.
   wp_loadField.
   iDestruct (is_slice_to_small with "Hreq_sl") as "Hreq_sl".
 
+  iMod (own_alloc (DfracOwn 1)) as (γreq) "HreqTok".
+  { done. }
   (* Put the EnterNewEpoch into an invariant now, os we  *)
   set (prophErrCode:=if prophErr then (U64 1) else (U64 0)).
-  iAssert (|={⊤}=> Get_req_inv prophVal prophErrCode e γ _
+  iAssert (|={⊤}=> Get_req_inv prophVal prophErrCode e γ γreq
                               (λ err v, if (decide (err = 0)) then Φ #v else True)
-          )%I with "[Hupd]" as ">#HgetInv".
+          )%I with "[Hupd HreqTok]" as ">#HgetInv".
   {
     rewrite /Get_req_inv.
-    iMod (inv_alloc getN  with "[Hupd]") as "$"; last done.
+    iMod (inv_alloc getN  with "[Hupd HreqTok]") as "$"; last done.
     iNext.
     iLeft.
-    (* FIXME: don't want to have to open up EnterNewEpoch_spec here *)
+    iFrame "HreqTok".
     (* Have f(P) in ctx. Want to prove f(Q). Want to know that it's enough to
        show that P -∗ Q. Basically, want to insist that a spec is covariant
        in its Φ argument (or maybe it's contravariant?). *)
-    rewrite /EnterNewEpoch_spec.
+    iApply (EnterNewEpoch_spec_wand with "[] Hupd").
+    iIntros "Hupd".
+    rewrite /Get_server_spec.
     iMod "Hupd".
     iModIntro.
     iDestruct "Hupd" as (?) "Hupd".
     iExists latestEpoch.
-    destruct (decide (int.Z latestEpoch < int.Z e)).
-    {
-      iDestruct "Hupd" as "($ & $ & Hupd)".
-      iIntros (?) "H1 H2 H3".
-      iMod ("Hupd" $! v with "H1 H2 H3") as "Hupd".
-      iModIntro.
+    iDestruct "Hupd" as "[$ Hupd]".
 
-      (* This is where the boring part ends. *)
-      rewrite /Get_server_spec.
+    destruct (decide (int.Z latestEpoch = int.Z e)).
+    {
+      rewrite /Get_core_spec.
       iMod "Hupd".
       iModIntro.
-      clear latestEpoch l.
-      iDestruct "Hupd" as (?) "Hupd".
-      iExists latestEpoch.
-      iDestruct "Hupd" as "[$ Hupd]".
+      iDestruct "Hupd" as (?) "[H1 Hupd]".
+      iExists _; iFrame "H1".
+      iIntros "H1".
+      iMod ("Hupd" with "H1") as "Hupd".
+      iModIntro.
 
-      destruct (decide (int.Z latestEpoch = int.Z e)).
-      {
-        rewrite /Get_core_spec.
-        iMod "Hupd".
-        iModIntro.
-        iDestruct "Hupd" as (?) "[H1 Hupd]".
-        iExists _; iFrame "H1".
-        iIntros "H1".
-        iMod ("Hupd" with "H1") as "Hupd".
-        iModIntro.
-
-        iIntros "H1".
-        iMod ("Hupd" with "H1") as "Hupd".
-        iModIntro.
-        iFrame "Hupd".
-      }
-      {
-        iIntros "H1".
-        iMod ("Hupd" with "H1") as "Hupd".
-        iModIntro.
-        iIntros.
-        iFrame.
-      }
+      iIntros "H1".
+      iMod ("Hupd" with "H1") as "Hupd".
+      iModIntro.
+      iFrame "Hupd".
     }
-    (* more boring proof where we show that EnterNewEpoch is covariant in Φ *)
-    admit.
+    {
+      iIntros "H1".
+      iMod ("Hupd" with "H1") as "Hupd".
+      iModIntro.
+      iIntros.
+      iFrame.
+    }
   }
 
   wp_apply (wp_Client__Call _ _ _ _ _ _ _ _ _ _
@@ -492,8 +510,7 @@ Proof.
 
   wp_loadField.
   destruct (decide (int.Z err = 0)).
-  {
-    (* no error *)
+  { (* no error *)
     replace (err) with (U64 0) by word.
     wp_pures.
     rewrite bool_decide_true; last done.
@@ -503,8 +520,9 @@ Proof.
     wp_apply (wp_ResolveProph_once (T:=bool) with "[Hprophe]").
     { done. }
     { iFrame. }
-    iIntros (_).
+    iIntros "%HprophErrFalse".
     iEval (simpl) in "Hpost".
+    iDestruct "Hpost" as "#Hpost".
 
     wp_pures.
     wp_loadField.
@@ -513,132 +531,58 @@ Proof.
     wp_apply (wp_ResolveProph_once (T:=u64) with "[$Hprophv]").
     { done. }
     iIntros "%HprophMatches".
-    wp_pures.
-    iApply wp_fupd.
-    wp_loadField.
+    (* XXX: some later hacking. Open the invariant here so we can strip off a later from the Φ. *)
+    iApply fupd_wp.
+
     (* Open HgetInv and use receipt to get Φ. *)
-    admit.
-  (*
-    iAssert
-      (|={⊤,∅}=> ∃ latestEpoch, if decide (int.Z latestEpoch < int.Z e)%Z then
-      own_latest_epoch γ latestEpoch (1/2)%Qp ∗
-      own_unused_epoch γ e ∗
-                            (∀ v, own_val γ e v (1/2)%Qp ∗
-                                           own_val γ latestEpoch v (1/2)%Qp ∗
-                                           own_latest_epoch γ e (1/2)%Qp
-                                           ={∅,⊤}=∗ (own_Clerk γ ck -∗ Φ #v))
-   else if decide (int.Z latestEpoch = int.Z e) then
-    ∃ v, own_latest_epoch γ latestEpoch (1/2)%Qp ∗
-     own_val γ e v (1/2)%Qp ∗
-    (own_val γ e v (1/2)%Qp ∗ own_latest_epoch γ e (1/2)%Qp ={∅,⊤}=∗ (own_Clerk γ ck -∗ Φ #v))
-   else
-     True)%I with "[]" as "Hupd".
-    { admit. } (* FIXME: will need to put this or the reply in escrow *)
-    simpl.
-    iExists valProph,errProph,_,_; iFrame "Hprophv".
-    iSplitL ""; first done.
-    iMod "Hupd".
-    iModIntro.
-    iDestruct "Hupd" as (latestEpoch) "Hupd".
-    iExists latestEpoch.
-    destruct (decide (int.Z latestEpoch < int.Z e)%Z).
+    iInv "HgetInv" as "Hi" "Hclose".
+    iDestruct "Hi" as "[[_ >Hbad] | [[_ >Hbad] | Hgood]]".
     {
-      iDestruct "Hupd" as "($ & $ & Hupd)".
-      iIntros (val) "Hpre".
-      iDestruct ("Hupd" with "Hpre") as "Hupd".
-      iMod "Hupd".
-      iModIntro.
-      iIntros.
-      iExists _,_.
-      iSplitL ""; first done.
-      setoid_rewrite decide_True; last done.
-      iFrame "Hupd".
-      iFrame.
+      iExFalso.
+      admit. (* op_receipt + unfinished -> False *)
     }
-    { (* similar to above *)
+    { (* Same as above *)
       admit.
     }
+    replace (prophErrCode) with (U64 0) by naive_solver.
+    (* XXX: I still don't know what setoid_rewrite does *)
+    iEval (setoid_rewrite decide_True) in "Hgood".
+    iMod ("Hclose" with "[]") as "_".
+    { (* FIXME: need another escrow token for taking Φ out of Get_req_inv *)
+      admit.
+    }
+    iModIntro.
+    wp_pures.
+    wp_loadField.
+    rewrite HprophMatches.
+    iDestruct "Hgood" as "[$ _]".
   }
-
-  iIntros (errCode) "(_ & Hreq_sl & Hpost)".
-  (* will be able to show that errCode = None iff err = false by prophecy.Resolve *)
-
-  wp_pures.
-  destruct errCode.
-  { (* case: error *)
+  { (* error; we'll exit in this case *)
+    wp_pures.
     rewrite bool_decide_false; last first.
-    { by destruct c. }
+    { naive_solver. }
+    simpl.
+
+    wp_apply (wp_ResolveProph_once (T:=bool) with "[$Hprophe]").
+    { done. }
+    iIntros "%HprophErrTrue".
+    wp_pures.
+    wp_loadField.
+    wp_pures.
+    rewrite bool_decide_false; last first.
+    { naive_solver. }
     wp_pures.
     wp_apply (wp_Exit).
     by iIntros.
-  (* FIXME: I don't know if I need to prophesize about the error code; if
-     there's an error, we just exit, and the caller finds out nothing *)
   }
-  (* case: no error *)
-  wp_pures.
-  iNamed "Hpost".
-  iDestruct "Hpost" as "(Hrep & Hrep_sl & Hpost)".
-  wp_load.
-  clear v.
-  clear err.
-  iDestruct "Hpost" as (v err) "(%Hrep_enc & Hpost)".
-
-  (* TODO: move this to a different lemma *)
-  wp_lam.
-  wp_apply (wp_new_dec with "Hrep_sl").
-  { done. }
-  iIntros (dec) "Hdec".
-  wp_pures.
-  wp_apply (wp_allocStruct).
-  { naive_solver. }
-  iIntros (r) "Hr".
-  iDestruct (struct_fields_split with "Hr") as "HH".
-  iNamed "HH".
-  simpl.
-  wp_pures.
-  wp_apply (wp_Dec__GetInt with "Hdec").
-  iIntros "Hdec".
-  wp_storeField.
-
-  wp_apply (wp_Dec__GetInt with "Hdec").
-  iIntros "Hdec".
-  wp_storeField.
-  wp_pures.
-  (* TODO: move the above to a different lemma *)
-  wp_loadField.
-  destruct (decide (int.Z err = 0)).
-  {
-    (* no error *)
-    replace (err) with (U64 0) by word.
-    wp_pures.
-    rewrite bool_decide_true; last done.
-    simpl.
-
-    (* maybe we don't need this *)
-    wp_apply (wp_ResolveProph_once (T:=bool) with "[]").
-    { admit. }
-    { admit. }
-    iIntros (_).
-
-    wp_pures.
-    wp_loadField.
-    wp_pures.
-    iDestruct "Hpost" as "[Hpost Hprophv]".
-    wp_loadField.
-    wp_apply (wp_ResolveProph_once (T:=u64) with "[$Hprophv]").
-    { done. }
-  } *)
 Admitted.
-
-
 
 Lemma wp_Server__Get γ s (e:u64) (rep:loc) (dummy_err dummy_val:u64) Post :
   is_Server γ s -∗
   {{{
         "Hrep_error" ∷ rep ↦[GetReply :: "err"] #dummy_err ∗
         "Hrep_val" ∷ rep ↦[GetReply :: "val"] #dummy_val ∗
-
-      "HgetSpec" ∷ EnterNewEpoch_spec γ e (Get_server_spec γ e Post)
+        "HgetSpec" ∷ EnterNewEpoch_spec γ e (Get_server_spec γ e Post)
   }}}
     Server__Get #s #e #rep
   {{{
